WIP SelArray

ulib/experimental/Steel.SelArray.fsti
@@ -11,7 +11,7 @@
    distributed under the License is distributed on an "AS IS" BASIS,
    WITHOUT WARRANTIES OR CONDITIONS OF ANY KIND, either express or implied.
    See the License for the specific language governing permissions and
-   limitations under the License.o
+   limitations under the License.
 *)
 
 module Steel.SelArray
@@ -20,18 +20,16 @@ open Steel.SelEffect
 open FStar.Ghost
 module U32 = FStar.UInt32
 
-let contents (t:Type u#0) = FStar.Seq.seq t
-let length #t (r:contents t) : GTot nat = Seq.length r
-
 val array (t:Type u#0) : Type u#0
+val length (#t: Type) (a: array t) : GTot nat
 
 val is_array (#a:Type0) (r:array a) : slprop u#1
-val array_sel (#a:Type0) (r:array a) : selector (contents a) (is_array r)
+val array_sel (#a:Type0) (r:array a) : selector (Seq.lseq a (length r)) (is_array r)
 
 [@@ __steel_reduce__]
 let varray' #a r : vprop' =
   {hp = is_array r;
-   t = Seq.seq a;
+   t = Seq.lseq a (length r);
    sel = array_sel r}
 
 [@@ __steel_reduce__]
@@ -41,37 +39,98 @@ let varray r = VUnit (varray' r)
 [@@ __steel_reduce__]
 let asel (#a:Type) (#p:vprop) (r:array a)
   (h:rmem p{FStar.Tactics.with_tactic selector_tactic (can_be_split p (varray r) /\ True)})
+: GTot (Seq.lseq a (length r))
   = h (varray r)
+
+
+(* Splitting an array (inspired from Steel.Array) *)
+
+noextract
+val boundary: Type0
+
+val lhs
+  (#t: Type)
+  (r: array t)
+: GTot boundary
+
+val rhs
+  (#t: Type)
+  (r: array t)
+: GTot boundary
+
+let adjacent
+  (#t: Type)
+  (al ar: array t)
+: Tot prop
+= rhs al == lhs ar
+
+val freeable_boundaries (lhs rhs: boundary) : GTot bool
+
+let freeable (#t: Type) (a: array t) : GTot bool =
+  freeable_boundaries (lhs a) (rhs a)
+
+val join (#t:Type) (al ar:array t)
+  : SteelSel (array t)
+          (varray al `star` varray ar)
+          (fun a -> varray a)
+          (fun _ -> adjacent al ar)
+          (fun h a h' ->
+            let s = h' (varray a) in
+            s == (h (varray al) `Seq.append` h (varray ar)) /\
+            lhs a == lhs al /\
+            rhs a == rhs ar
+          )
+
+val split (#t:Type) (a:array t) (i:U32.t)
+  : SteelSel (array t & array t)
+          (varray a)
+          (fun res -> varray (fst res) `star` varray (snd res))
+          (fun _ -> U32.v i <= length a)
+          (fun h (al, ar) h' ->
+            let s = h (varray a) in
+            let sl = h' (varray al) in
+            let sr = h' (varray ar) in
+            U32.v i <= length a /\
+            adjacent al ar /\
+            lhs al == lhs a /\
+            rhs ar == rhs a /\
+            sl == Seq.slice s 0 (U32.v i) /\
+            sr == Seq.slice s (U32.v i) (length a)
+          )
 
 val alloc (#t:Type) (x:t) (n:U32.t)
   : SteelSel (array t)
              vemp
              (fun r -> varray r)
              (requires fun _ -> True)
-             (ensures fun _ r h1 -> asel r h1 == Seq.create (U32.v n) x)
+             (ensures fun _ r h1 ->
+               asel r h1 == Seq.create (U32.v n) x /\
+               freeable r
+             )
 
 val index (#t:Type) (r:array t) (i:U32.t)
   : SteelSel t
              (varray r)
              (fun _ -> varray r)
-             (requires fun h -> U32.v i < length (asel r h))
+             (requires fun _ -> U32.v i < length r)
              (ensures fun h0 x h1 ->
-               U32.v i < length (asel r h1) /\
-               asel r h0 == asel r h1 /\
-               x == Seq.index (asel r h1) (U32.v i))
+               let s = asel r h1 in
+               U32.v i < length r /\
+               asel r h0 == s /\
+               x == Seq.index s (U32.v i))
 
 val upd (#t:Type) (r:array t) (i:U32.t) (x:t)
   : SteelSel unit
              (varray r)
              (fun _ -> varray r)
-             (requires fun h -> U32.v i < length (asel r h))
+             (requires fun h -> U32.v i < length r)
              (ensures fun h0 _ h1 ->
-               U32.v i < length (asel r h0) /\
+               U32.v i < length r /\
                asel r h1 == Seq.upd (asel r h0) (U32.v i) x)
 
 val free (#t:Type) (r:array t)
   : SteelSel unit
              (varray r)
              (fun _ -> vemp)
-             (requires fun _ -> True)
+             (requires fun _ -> freeable r)
              (ensures fun _ _ _ -> True)
